add support for enums

jsonstar.schema.generation.test/SchemaGenerationTests.fs
@@ -8,93 +8,113 @@ type SchemaGenerationTests() =
     
     [<Test>]
     member this.StringSchema() =
-        let expected_schema_string = """{ "definitions" : {  }, "type" : "string" }"""
+        let expected_schema_string = """{ "type" : "string" }"""
         
         printfn "%s" SchemaExamples.schema_string
         Assert.AreEqual(expected_schema_string, SchemaExamples.schema_string)
 
     [<Test>]
     member this.IntSchema() =
-        let expected_schema_string = """{ "definitions" : {  }, "type" : "integer" }"""
+        let expected_schema_string = """{ "type" : "integer" }"""
         
         printfn "%s" SchemaExamples.schema_int
         Assert.AreEqual(expected_schema_string, SchemaExamples.schema_int)
 
     [<Test>]
     member this.BoolSchema() =
-        let expected_schema_string = """{ "definitions" : {  }, "type" : "boolean" }"""
+        let expected_schema_string = """{ "type" : "boolean" }"""
         
         printfn "%s" SchemaExamples.schema_bool
         Assert.AreEqual(expected_schema_string, SchemaExamples.schema_bool)
 
     [<Test>]
     member this.NatSchema() =
-        let expected_schema_string = """{ "definitions" : {  }, "minimum" : "0", "type" : "integer" }"""
+        let expected_schema_string = """{ "minimum" : "0", "type" : "integer" }"""
           
         printfn "%s" SchemaExamples.schema_nat
         Assert.AreEqual(expected_schema_string, SchemaExamples.schema_nat)
 
     [<Test>]
     member this.MoreThanOrEqualFiveSchema() =
-        let expected_schema_string = """{ "definitions" : {  }, "minimum" : "5", "type" : "integer" }"""
+        let expected_schema_string = """{ "minimum" : "5", "type" : "integer" }"""
         Assert.AreEqual(expected_schema_string, SchemaExamples.schema_moreThanOrEqualFive)
     
     [<Test>]
     member this.MoreThanFiveSchema() =
-        let expected_schema_string = """{ "definitions" : {  }, "minimum" : "6", "type" : "integer" }"""
+        let expected_schema_string = """{ "minimum" : "6", "type" : "integer" }"""
         Assert.AreEqual(expected_schema_string, SchemaExamples.schema_moreThanFive)
 
     [<Test>]
     member this.LessThanOrEqualFiveSchema() =
-        let expected_schema_string = """{ "definitions" : {  }, "maximum" : "5", "type" : "integer" }"""
+        let expected_schema_string = """{ "maximum" : "5", "type" : "integer" }"""
         Assert.AreEqual(expected_schema_string, SchemaExamples.schema_lessThanOrEqualFive)
 
     [<Test>]
     member this.LessThanFiveSchema() =
-        let expected_schema_string = """{ "definitions" : {  }, "maximum" : "4", "type" : "integer" }"""
+        let expected_schema_string = """{ "maximum" : "4", "type" : "integer" }"""
         Assert.AreEqual(expected_schema_string, SchemaExamples.schema_lessThanFive)
 
     [<Test>]
     member this.nat2Schema() =
-        let expected_schema_string = """{ "definitions" : {  }, "minimum" : "0", "type" : "integer" }"""
+        let expected_schema_string = """{ "minimum" : "0", "type" : "integer" }"""
         Assert.AreEqual(expected_schema_string, SchemaExamples.schema_nat2)
 
     [<Test>]
     member this.minimum3Schema() =
-        let expected_schema_string = """{ "definitions" : {  }, "minimum" : "3", "type" : "integer" }"""
+        let expected_schema_string = """{ "minimum" : "3", "type" : "integer" }"""
         Assert.AreEqual(expected_schema_string, SchemaExamples.schema_minimum3)
 
     [<Test>]
     member this.maximum8Schema() =
-        let expected_schema_string = """{ "definitions" : {  }, "maximum" : "8", "type" : "integer" }"""
+        let expected_schema_string = """{ "maximum" : "8", "type" : "integer" }"""
         Assert.AreEqual(expected_schema_string, SchemaExamples.schema_maximum8)
 
     [<Test>]
     member this.min5max9Schema() =
-        let expected_schema_string = """{ "definitions" : {  }, "minimum" : "5", "maximum" : "9", "type" : "integer" }"""
+        let expected_schema_string = """{ "minimum" : "5", "maximum" : "9", "type" : "integer" }"""
         Assert.AreEqual(expected_schema_string, SchemaExamples.schema_min5max9)
 
     [<Test>]
     member this.min5max9dslSchema() =
-        let expected_schema_string = """{ "definitions" : {  }, "minimum" : "5", "maximum" : "9", "type" : "integer" }"""
+        let expected_schema_string = """{ "minimum" : "5", "maximum" : "9", "type" : "integer" }"""
         Assert.AreEqual(expected_schema_string, SchemaExamples.schema_min5max9dsl)
 
     [<Test>]
     member this.string_max5Schema() =
-        let expected_schema_string = """{ "definitions" : {  }, "maxLength" : "5", "type" : "string" }"""
+        let expected_schema_string = """{ "maxLength" : "5", "type" : "string" }"""
         Assert.AreEqual(expected_schema_string, SchemaExamples.schema_string_max5)
 
     [<Test>]
     member this.string_min3max5Schema() =
-        let expected_schema_string = """{ "definitions" : {  }, "maxLength" : "5", "minLength" : "3", "type" : "string" }"""
+        let expected_schema_string = """{ "maxLength" : "5", "minLength" : "3", "type" : "string" }"""
         Assert.AreEqual(expected_schema_string, SchemaExamples.schema_string_min3max5)
 
     [<Test>]
     member this.string_max5dslSchema() =
-        let expected_schema_string = """{ "definitions" : {  }, "maxLength" : "5", "type" : "string" }"""
+        let expected_schema_string = """{ "maxLength" : "5", "type" : "string" }"""
         Assert.AreEqual(expected_schema_string, SchemaExamples.schema_string_max5_dsl)
 
     [<Test>]
     member this.string_min3max5dslSchema() =
-        let expected_schema_string = """{ "definitions" : {  }, "maxLength" : "5", "minLength" : "3", "type" : "string" }"""
+        let expected_schema_string = """{ "maxLength" : "5", "minLength" : "3", "type" : "string" }"""
         Assert.AreEqual(expected_schema_string, SchemaExamples.schema_string_min3max5_dsl)
+
+    [<Test>]
+    member this.enum_onetwothreeSchema() =
+        let expected_schema_string = """{ "enum" : [ "One", "Two", "Three" ], "type" : "string" }"""
+        Assert.AreEqual(expected_schema_string, SchemaExamples.schema_enum_onetwothree)
+
+    [<Test>]
+    member this.enum_onetwoonlySchema() =
+        let expected_schema_string = """{ "enum" : [ "One", "Two" ], "type" : "string" }"""
+        Assert.AreEqual(expected_schema_string, SchemaExamples.schema_enum_onetwoonly)
+
+    [<Test>]
+    member this.enum_withouttwoSchema() =
+        let expected_schema_string = """{ "enum" : [ "One", "Three" ], "type" : "string" }"""
+        Assert.AreEqual(expected_schema_string, SchemaExamples.schema_enum_withouttwo)
+
+    [<Test>]
+    member this.enum_onetwoonly_withoutoneSchema() =
+        let expected_schema_string = """{ "enum" : [ "Two" ], "type" : "string" }"""
+        Assert.AreEqual(expected_schema_string, SchemaExamples.schema_enum_onetwoonly_withoutone)
