jsonstar/JsonStar.Schema.Generation.Recognizers.fst
@@ -8,11 +8,39 @@ let primitives = [ "Prims.string"; "Prims.int"; "Prims.bool" ]
 type term_type = 
     | Primitive : t:T.term -> term_type
     | Refinement : t:T.term -> term_type
+    | Enum : t:T.fv -> term_type
     | Unrecognized : t:T.term -> term_type
+
+val satisfy_all: ('a -> T.Tac bool) -> list 'a -> T.Tac bool
+let rec satisfy_all f x = match x with
+  | [] -> true
+  | a::tl -> if f a then satisfy_all f tl else false
+
+let isEnum (fv : T.fv) : T.Tac bool = 
+    let env = T.cur_env () in
+    let qname = T.inspect_fv fv in
+    match T.lookup_typ env qname with
+    | Some s -> begin
+        // Check if sig in an enum definition
+        match T.inspect_sigelt s with
+        | T.Sg_Let _ _ _ _ _ -> false
+        | T.Sg_Inductive _ _ _ _ cts -> begin
+            // check if all constructor types are simply the type of the enum
+            satisfy_all (fun (_, ct) -> Helpers.termeq (T.pack (T.Tv_FVar fv)) ct) cts
+            end
+        | T.Unk -> false // TODO: What's Unk? Should we fail here?
+        end
+    | None -> false
 
 let term_to_type (t : T.term) : T.Tac term_type =
     let tv : T.term_view = T.inspect t in
     match tv with 
-    | T.Tv_FVar fv when L.mem (T.fv_to_string fv) primitives -> Primitive t
+    | T.Tv_FVar fv -> begin
+        if L.mem (T.fv_to_string fv) primitives then 
+            Primitive t
+        else if isEnum fv then
+            Enum fv
+        else Unrecognized t
+        end
     | T.Tv_Refine _ _ -> Refinement t
     | _               -> Unrecognized t
