jsonstar.schema.generation.test/SchemaDslTests.fst
@@ -1,0 +1,30 @@
+module SchemaDslTests
+
+open Types
+
+open JsonStar.Schema.Dsl
+
+// positive tests
+let nat2_p_ex1 : nat2 = 5
+let minimum3_p_ex1 : minimum3 = 3
+let maximum8_p_ex1 : maximum8 = 8
+
+let min5max9_p_ex1 : min5max9 = 5
+let min5max9_p_ex2 : min5max9 = 9
+
+
+
+// negative tests
+[@@(expect_failure [19])]
+let nat2_n_ex1 : nat2 = -1
+
+[@@(expect_failure [19])]
+let minimum3_n_ex1 : minimum3 = 2
+
+[@@(expect_failure [19])]
+let maximum8_n_ex1 : maximum8 = 9
+
+[@@(expect_failure [19])]
+let min5max9_n_ex1 : min5max9 = 4
+[@@(expect_failure [19])]
+let min5max9_n_ex2 : min5max9 = 10
