jsonstar.schema.generation.test/SchemaExamples.fst
@@ -1,22 +1,6 @@
 ﻿module SchemaExamples
 
-type lessThanOrEqualFive = x:int{x <= 5}
-type lessThanFive = x:int{x < 5}
-type moreThanOrEqualFive = x:int{x >= 5}
-type moreThanFive = x:int{x > 5}
-
-type nat2 = x:int{JsonStar.Schema.Dsl.minimum x 0}
-type minimum3 = x:int{JsonStar.Schema.Dsl.minimum x 3}
-type maximum8 = x:int{JsonStar.Schema.Dsl.maximum x 8}
-
-let min5max9 = x:int{x >= 5 && x <= 9}
-let min5max9dsl = x:int{JsonStar.Schema.Dsl.minimum x 5 && JsonStar.Schema.Dsl.maximum x 9}
-
-type string_max5 = s:string{String.length s <= 5}
-type string_min3max5 = s:string{String.length s >= 3 && String.length s <= 5}
-
-type string_max5_dsl = s:string{JsonStar.Schema.Dsl.maxLength s 5}
-type string_min3max5_dsl = s:string{JsonStar.Schema.Dsl.minLength s 3 && JsonStar.Schema.Dsl.maxLength s 5}
+open Types
 
 let schema_string : string = 
     let s : JsonStar.Schema.schema = (FStar.Tactics.synth_by_tactic (fun () -> JsonStar.Schema.Generation.gen_schema FStar.Tactics.Goal (`string))) in
@@ -84,4 +68,20 @@ let schema_string_max5_dsl =
 
 let schema_string_min3max5_dsl =
     let s : JsonStar.Schema.schema = (FStar.Tactics.synth_by_tactic (fun () -> JsonStar.Schema.Generation.gen_schema FStar.Tactics.Goal (`string_min3max5_dsl))) in
+    JsonStar.PrettyPrint.stringify (JsonStar.Schema.toJson s)
+
+let schema_enum_onetwothree =
+    let s : JsonStar.Schema.schema = (FStar.Tactics.synth_by_tactic (fun () -> JsonStar.Schema.Generation.gen_schema FStar.Tactics.Goal (`enum_onetwothree))) in
+    JsonStar.PrettyPrint.stringify (JsonStar.Schema.toJson s)
+
+let schema_enum_onetwoonly =
+    let s : JsonStar.Schema.schema = (FStar.Tactics.synth_by_tactic (fun () -> JsonStar.Schema.Generation.gen_schema FStar.Tactics.Goal (`enum_onetwoonly))) in
+    JsonStar.PrettyPrint.stringify (JsonStar.Schema.toJson s)
+
+let schema_enum_withouttwo =
+    let s : JsonStar.Schema.schema = (FStar.Tactics.synth_by_tactic (fun () -> JsonStar.Schema.Generation.gen_schema FStar.Tactics.Goal (`enum_withouttwo))) in
+    JsonStar.PrettyPrint.stringify (JsonStar.Schema.toJson s)
+
+let schema_enum_onetwoonly_withoutone =
+    let s : JsonStar.Schema.schema = (FStar.Tactics.synth_by_tactic (fun () -> JsonStar.Schema.Generation.gen_schema FStar.Tactics.Goal (`enum_onetwoonly_withoutone))) in
     JsonStar.PrettyPrint.stringify (JsonStar.Schema.toJson s)
