jsonstar.schema.generation.test/Types.fst
@@ -1,0 +1,31 @@
+module Types
+
+module SchemaDsl = JsonStar.Schema.Dsl
+
+type lessThanOrEqualFive = x:int{x <= 5}
+type lessThanFive = x:int{x < 5}
+type moreThanOrEqualFive = x:int{x >= 5}
+type moreThanFive = x:int{x > 5}
+
+type nat2 = x:int{JsonStar.Schema.Dsl.minimum x 0}
+type minimum3 = x:int{JsonStar.Schema.Dsl.minimum x 3}
+type maximum8 = x:int{JsonStar.Schema.Dsl.maximum x 8}
+
+let min5max9 = x:int{x >= 5 && x <= 9}
+let min5max9dsl = x:int{JsonStar.Schema.Dsl.minimum x 5 && JsonStar.Schema.Dsl.maximum x 9}
+
+type string_max5 = s:string{String.length s <= 5}
+type string_min3max5 = s:string{String.length s >= 3 && String.length s <= 5}
+
+type string_max5_dsl = s:string{JsonStar.Schema.Dsl.maxLength s 5}
+type string_min3max5_dsl = s:string{JsonStar.Schema.Dsl.minLength s 3 && JsonStar.Schema.Dsl.maxLength s 5}
+
+type enum_onetwothree = 
+    | One
+    | Two
+    | Three
+    
+type enum_onetwoonly = x:enum_onetwothree{ SchemaDsl.allow x [ One?; Two?; ]}
+type enum_withouttwo = x:enum_onetwothree{ SchemaDsl.disallow x [ Two?; ]}
+
+type enum_onetwoonly_withoutone = x:enum_onetwoonly{ SchemaDsl.disallow x [ One?;] }
