jsonstar/JsonStar.Schema.Dsl.fst
@@ -9,11 +9,17 @@ NOTE: Functions marked as irreducible can't be replaced with it's implementation
 TODO: Does this break automatic F* proves similarly to hiding the implementation behind the interface?
 *)
 
+(*
+NOTE: The convention here is that the first argument is always the value we're restricting, e.g.
+for "s:string{minLength s 5}" it is 's'.
+*)
+
 // string options
 let minLength (s : string) (n : nat) = String.length s >= n
 let maxLength (s : string) (n : nat) = String.length s <= n
-// TODO: Stub only - add real pattern matching
-let pattern (s : string) (p : string) = true
+// TODO: Stub only - add real pattern matching. 
+// Irreducible can be removed when some implementation is provided, as currently F* simplifies it to just C_True
+irreducible let pattern (s : string) (p : string) = true
 // TODO: How do we handle 'reference'? DSL or attribute?
 
 // number options
@@ -23,9 +29,21 @@ let maximum (x : int) (n : int) = x <= n
 // Object options
 
 // Array options
-irreducible let minItems (l : list 'a) (n : nat) = List.Tot.length l >= n
-irreducible let maxItems (l : list 'a) (n : nat) = List.Tot.length l <= n
-irreducible let uniqueItems (#a:eqtype) (l : list a) = List.Tot.noRepeats l
+let minItems (l : list 'a) (n : nat) = List.Tot.length l >= n
+let maxItems (l : list 'a) (n : nat) = List.Tot.length l <= n
+let uniqueItems (#a:eqtype) (l : list a) = List.Tot.noRepeats l
+
+// enum options
+/// Restricts enum to only allow certain values from the list
+irreducible let rec allow (x : 'a) (l : list ('a -> bool)) = 
+    match l with
+    | [] -> false
+    | f :: fs -> if f x then true else allow x fs
+/// Restricts enum so that certain values are not allowed
+let rec disallow (x : 'a) (l : list ('a -> bool)) = 
+    match l with
+    | [] -> true
+    | f :: fs -> if f x then false else disallow x fs
 
 // TODO: Decide how do we want to express "oneOf" and "dependencies"
 
