jsonstar/JsonStar.Schema.Generation.Api.fst
@@ -16,8 +16,25 @@ let nat2_s : schema = T.synth_by_tactic (fun () -> SchemaGen.gen_schema T.Goal (
 let min5max9 = x:int{x >= 5 && x <= 9}
 let min5max9_s : schema = T.synth_by_tactic (fun () -> SchemaGen.gen_schema T.Goal (`min5max9))
 
-type string_max5 = s:string{JsonStar.Schema.Dsl.maxLength s 5}
+type string_max5 = s:string{SchemaDsl.maxLength s 5}
 let string_max5_s : schema = T.synth_by_tactic (fun () -> SchemaGen.gen_schema T.Goal (`string_max5))
 
-type string_min3max5 = s:string{JsonStar.Schema.Dsl.minLength s 3 && JsonStar.Schema.Dsl.maxLength s 5}
+type string_min3max5 = s:string{SchemaDsl.minLength s 3 && SchemaDsl.maxLength s 5}
 let string_min3max5_s : schema = T.synth_by_tactic (fun () -> SchemaGen.gen_schema T.Goal (`string_min3max5))
+
+type string_pat = s:string{SchemaDsl.pattern s "YYYY-MM-DD"}
+let string_pat_s : schema = T.synth_by_tactic (fun () -> SchemaGen.gen_schema T.Goal (`string_pat))
+
+type enum_onetwothree = 
+    | One
+    | Two
+    | Three
+let enum_onetwothree_s : schema = T.synth_by_tactic (fun () -> SchemaGen.gen_schema T.Goal (`enum_onetwothree))
+
+//let x : enum_onetwothree = T.synth_by_tactic (fun () -> SchemaGen.print_term T.Goal (`One))
+
+type enum_onetwoonly = x:enum_onetwothree{ SchemaDsl.allow x [ One?; Two?; ]}
+type enum_withoutthree = x:enum_onetwothree{ SchemaDsl.disallow x [ Two?; ]}
+
+let enum_onetwoonly_s : schema = T.synth_by_tactic (fun () -> SchemaGen.gen_schema T.Goal (`enum_onetwoonly))
+let enum_withoutthree_s : schema = T.synth_by_tactic (fun () -> SchemaGen.gen_schema T.Goal (`enum_withoutthree))
