jsonstar/JsonStar.Schema.Generation.Refinement.fst
@@ -23,6 +23,10 @@ type string_refinement =
     | MaxLength : v:nat -> string_refinement
     | Pattern : v:string -> string_refinement
 
+type enum_refinement = 
+    | Allow : v:list string -> enum_refinement
+    | Disallow : v:list string -> enum_refinement
+
 type complex_refinement = 
     // Tv_App (op_And x1, x2)
     | And : x1:T.term -> x2:T.term -> complex_refinement
@@ -32,26 +36,50 @@ let intFromTerm (t : T.term) : T.Tac int =
     | T.Tv_Const (T.C_Int x) -> x
     | _ -> Helpers.tfail ("Expected integer. Got " ^ (T.term_to_string t) ^ ".\n")
 
-// Extracts the operator
-let numberRefinementFromTerm (ref : T.term) (value : T.term) : T.Tac number_refinement =
-    let v = intFromTerm value in
-    match T.inspect ref with
-    | T.Tv_App op _ -> begin
-        if op `Helpers.termeq` (`Prims.op_GreaterThanOrEqual) then Minimum v
-        else if op `Helpers.termeq` (`Prims.op_GreaterThan) then Minimum (v + 1)
-        else if op `Helpers.termeq` (`Prims.op_LessThanOrEqual) then Maximum v
-        else if op `Helpers.termeq` (`Prims.op_LessThan) then Maximum (v - 1)
-        else Helpers.tfail ("Unrecognized operator: " ^ (T.term_to_string op) ^ ".\n")
-        end
-    | _ -> Helpers.tfail ("Expected operator. Got " ^ (T.term_to_string ref) ^ ".\n")
+// A helper functions for dropping arguments from DSL functions except the one which represents the
+// restricted value (assumed to always be the first argument in DSL function).
+// `dsl_fun should result in something like:
+// Abs (Abs (App (App ref ref_val)))
+// where ref is the implementation of our DSL function, and ref_val is the argument we are refining.
+// We want to retain "App ref ref_val" and use it for comparisons as it's the biggest unchanging part 
+// within the Tv_Refine we're getting as input. 
+let dropExtraArgs (t : T.term) : T.Tac T.term =
+    let rec dropArgsAux (t : T.term) (n : nat) : T.Tac T.term = 
+        match T.inspect t with
+        | T.Tv_Abs _ t1 -> dropArgsAux t1 (n + 1)
+        | T.Tv_App t _ -> if n > 2 then dropArgsAux t (n-1) else t
+        | _ -> T.fail ("Expected either Abs or App. Got " ^ (T.term_to_string t))
+    in
+    dropArgsAux t 0
 
-// We need to extract the refinement from the term representation of a DSL function. 
-// This means dropping the abstractions (function arguments) and a top-level application
-let rec dslToRef (t : T.term) : T.Tac T.term = 
-    match T.inspect t with
-    | T.Tv_Abs _ t1 -> dslToRef t1
-    | T.Tv_App t _ -> t
-    | _ -> t
+// For DSL functions we need to first expand their name and then drop extra arguments as we only need to recognize 
+// that a certain function was used in the refinement.
+let dslToRef (t : T.term) : T.Tac T.term = dropExtraArgs (T.norm_term_env (T.cur_env()) [delta] t)
+
+// Extracts the operator
+let numberRefinementFromTerm (ref : T.term) : T.Tac number_refinement =
+    // Number refinements take two arguments. The first one is assumed to always be the refined number
+    // and the second a value by which we restrict it.
+    match T.inspect ref with
+    | T.Tv_App op_with_arg (value, _) -> begin
+        let v = intFromTerm value in
+        // We need to drop the first argument now
+        match T.inspect op_with_arg with
+        | T.Tv_App op _ -> begin
+            //T.print "NumberRef";
+            //Helpers.printAst op;
+            //Helpers.printAst (`Prims.op_GreaterThanOrEqual);
+
+            // Number refinements are very simple so there's no point in adding extra support for irreducible case
+            if op `Helpers.termeq` (`Prims.op_GreaterThanOrEqual) then Minimum v
+            else if op `Helpers.termeq` (`Prims.op_GreaterThan) then Minimum (v + 1)
+            else if op `Helpers.termeq` (`Prims.op_LessThanOrEqual) then Maximum v
+            else if op `Helpers.termeq` (`Prims.op_LessThan) then Maximum (v - 1)
+            else Helpers.tfail ("Unrecognized operator: " ^ (T.term_to_string op) ^ ".\n")
+            end
+        | _ -> Helpers.tfail ("Expected operator with argument. Got " ^ (T.term_to_string op_with_arg) ^ ".\n")
+        end
+    | _ -> Helpers.tfail ((T.term_to_string ref) ^ " expected to be of form Tv_App op value where op describes refinement and value is the value that should be used.")
 
 // NOTE: We can easily match against DSL, if we forbid F* from unfolding it. Unfortunately,
 //       marking the DSL functions as "irreducible" or hiding them behind the interface has an 
@@ -64,27 +92,41 @@ let rec dslToRef (t : T.term) : T.Tac T.term =
 //       not easy to match against unfolded representation, it's possible to mark a certain function 
 //       as irreducible and carry on with recognizing the name as below (DSL section). But one needs to 
 //       keep in mind it will become harder to use on the client side. 
-let stringRefinementFromTerm (ref : T.term) (value : T.term) : T.Tac string_refinement =
-    //T.print "stringref";
-    //Helpers.printAst ref;
-    //Helpers.printAst (dslToRef (Helpers.drop_synonym (T.top_env()) (`(JsonStar.Schema.Dsl.maxLength))));
-    if ref `Helpers.termeq` (dslToRef (Helpers.drop_synonym (T.top_env()) (`(JsonStar.Schema.Dsl.maxLength))))
-        then MaxLength (T.unquote value)
-    else if ref `Helpers.termeq` (dslToRef (Helpers.drop_synonym (T.top_env()) (`(JsonStar.Schema.Dsl.minLength))))
-        then MinLength (T.unquote value)
-    else if ref `Helpers.termeq` (dslToRef (Helpers.drop_synonym (T.top_env()) (`(JsonStar.Schema.Dsl.pattern))))
-        then Pattern (T.unquote value)
-    else begin
-        // try matching DSL
-        match T.inspect ref with
-        | T.Tv_App op _ -> begin
-            if op `Helpers.termeq` (`JsonStar.Schema.Dsl.maxLength) then MaxLength (T.unquote value)
-            else if op `Helpers.termeq` (`JsonStar.Schema.Dsl.minLength) then MinLength (T.unquote value)
-            else if op `Helpers.termeq` (`JsonStar.Schema.Dsl.pattern) then Pattern (T.unquote value)
-            else Helpers.tfail ("Unrecognized string operator: " ^ (T.term_to_string op) ^ ".\n")
+let stringRefinementFromTerm (ref : T.term) : T.Tac string_refinement =
+    // In the irreducible case "ref" comes as a function name and it's arguments. There's one 
+    // Tv_App per argument, e.g. 
+    // Tv_App (Tv_App (Tv_FVar JsonStar.Schema.Dsl.pattern, Tv_Var (s:Prims.string)), C_String YYYY-MM-DD)
+    // String refinements take two arguments. The first one is assumed to always be the refined string
+    // and the second a value by which we restrict it.
+    match T.inspect ref with
+    | T.Tv_App op_with_arg (value, _) -> begin
+        match T.inspect op_with_arg with
+        | T.Tv_App op_dsl _ -> begin
+            //T.print "stringop_irreducible";
+            //Helpers.printAst op_dsl;
+            //Helpers.printAst (`JsonStar.Schema.Dsl.maxLength);
+            //Helpers.printAst (`JsonStar.Schema.Dsl.minLength);
+            //Helpers.printAst (`JsonStar.Schema.Dsl.pattern);
+
+            // Try matching against DSL first (irreducible functions)
+            if op_dsl `Helpers.termeq` (`JsonStar.Schema.Dsl.maxLength) then MaxLength (T.unquote value)
+            else if op_dsl `Helpers.termeq` (`JsonStar.Schema.Dsl.minLength) then MinLength (T.unquote value)
+            else if op_dsl `Helpers.termeq` (`JsonStar.Schema.Dsl.pattern) then Pattern (T.unquote value)
+            else begin
+                //T.print "stringop";
+                //Helpers.printAst op_with_arg;
+                //Helpers.printAst (dslToRef (`JsonStar.Schema.Dsl.maxLength));
+                //Helpers.printAst (dslToRef (`JsonStar.Schema.Dsl.minLength));
+                ////Helpers.printAst (dslToRef (`JsonStar.Schema.Dsl.pattern)); //pattern is irreducible currently, so this line would fail
+
+                if op_with_arg `Helpers.termeq` (dslToRef (`JsonStar.Schema.Dsl.maxLength)) then MaxLength (T.unquote value)
+                else if op_with_arg `Helpers.termeq` (dslToRef (`JsonStar.Schema.Dsl.minLength)) then MinLength (T.unquote value)
+                else if op_with_arg `Helpers.termeq` (dslToRef (`JsonStar.Schema.Dsl.pattern)) then Pattern (T.unquote value)
+                else Helpers.tfail ("Unrecognized string operator: " ^ (T.term_to_string op_with_arg) ^ ".\n")
+                end
             end
-        | _ -> Helpers.tfail ("Expected string restriction. Got " ^ (T.term_to_string ref) ^ ".\n")
-    end
+        end
+    | _ -> Helpers.tfail ((T.term_to_string ref) ^ " expected to be of form Tv_App op value where op describes refinement and value is the value that should be used.")
 
 let tryComplexFromTerm (t : T.term) : T.Tac (option complex_refinement) = 
     match T.inspect t with
@@ -92,7 +134,8 @@ let tryComplexFromTerm (t : T.term) : T.Tac (option complex_refinement) =
     | T.Tv_App l (x2, _) -> begin
         match T.inspect l with
         | T.Tv_App op (x1, _) ->
-            if op `Helpers.termeq` (`Prims.op_AmpAmp)
+            // TODO: Use Helpers.termeq consistently
+            if op `T.term_eq` (`Prims.op_AmpAmp)
                 then Some (And x1 x2)
                 else None
         | _ -> None
@@ -105,7 +148,7 @@ let dropTopLevelEqTrue (t : T.term) : T.Tac T.term =
     | T.Comp (T.Eq _) l _ -> l
     | _ -> t
 
-let rec refinementsFromTerm (refinementFromTerm : T.term -> T.term -> T.Tac 'a) (t : T.term) : T.Tac (list 'a) =
+let rec refinementsFromTerm (refinementFromTerm : T.term -> T.Tac 'a) (t : T.term) : T.Tac (list 'a) =
     //Helpers.printAst t;
     let t = (dropTopLevelEqTrue t) in
     // Check if this is a complex refinement
@@ -119,19 +162,71 @@ let rec refinementsFromTerm (refinementFromTerm : T.term -> T.term -> T.Tac 'a) 
         let refs = List.Tot.append refs_left refs_right in
         refs
         end
-    | None -> begin 
+    | None -> 
         // fallback to single refinement
-        match T.inspect t with
-        | T.Tv_App op value -> begin
-            let ref = refinementFromTerm op (fst value) in
-            [ ref ]
-            end
-        | _ -> Helpers.tfail ((T.term_to_string t) ^ " is not supported refinement.\n")
-        end
+        [ refinementFromTerm t ]
 
-let rec numberRefinementsFromTerm (t : T.term) : T.Tac (list number_refinement) =
+let numberRefinementsFromTerm (t : T.term) : T.Tac (list number_refinement) =
     refinementsFromTerm numberRefinementFromTerm t
 
-let rec stringRefinementsFromTerm (t : T.term) : T.Tac (list string_refinement) = 
+let stringRefinementsFromTerm (t : T.term) : T.Tac (list string_refinement) = 
     refinementsFromTerm stringRefinementFromTerm t
+    
+let enumRefinementFromTerm (t : T.term) : T.Tac enum_refinement = 
+    let t = (dropTopLevelEqTrue t) in
+    // Check if this is a complex refinement
+    match tryComplexFromTerm t with
+    | Some (And t1 t2) -> Helpers.tfail ("Only single refinement on enum is supported.")
+    | None -> begin
+        // In the irreducible case "ref" comes as a function name and it's arguments. There's one 
+        // Tv_App per argument, e.g. 
+        // Tv_App (Tv_App (Tv_FVar JsonStar.Schema.Dsl.allow, Tv_Var (x:some_enum_type)), list_of_projectors)
+        // Enum refinements take two arguments. The first one is assumed to always be the refined enum
+        // and the second a list of constructors which we use to restrict it.
+
+        // For enums we're interested only in figuring out that SchemaDsl.allow is used. 
+        // With a refinement like: "x:enum_onetwothree{ SchemaDsl.allow x _}" where "_" is some list of allowed constructors we get
+        // (Tv_App (Tv_FVar JsonStar.Schema.Dsl.allow, Tv_FVar JsonStar.Schema.Generation.Api.enum_onetwothree), Tv_Var (x:JsonStar.Schema.Generation.Api.enum_onetwothree))
+        // and we need to extract "Tv_FVar JsonStar.Schema.Dsl.allow".
+        // We can't match against "SchemaDsl.allow x" as in e.g. string refinements, as allow/disallow are implemented as visible recursive definitions 
+        // and delta normalization doesn't have any effect, and normalizing with zeta replaces the function with it's implementation in terms of match statement.  
+        match T.inspect t with
+        | T.Tv_App op_with_arg (value, _) -> begin
+            // 1. Extract constructors from the enum type
+            // 2. Use value to get a list of selectors
+            // 3. Evaluate constructors on a list of selectors - filter those for which some selector returns true
+            // 4. Convert constructors to their names
+            // 5. Return as value of the restriction
+
+            match T.inspect op_with_arg with
+            | T.Tv_App op_dsl _ -> begin
+                // Drop extra App
+                match T.inspect op_dsl with
+                | T.Tv_App op (enum_typ, _) -> begin
+                    let constructors = 
+                        match T.inspect enum_typ with
+                        | T.Tv_FVar fv -> begin
+                            let ctrs = JsonStar.Schema.Generation.Enum.get_enum_constructors fv in
+                            T.map (fun ctr -> Enum.pack_enum_constructor ctr) ctrs
+                            end
+                        | _ -> T.fail ("Expected an enum type. Got " ^ (T.term_to_ast_string enum_typ))
+                    in
+
+                    let selected_constructors = 
+                        let ty : Type = T.unquote enum_typ in
+                        let filtered_constructor_term : list ty = 
+                            T.filter_map (fun ctr -> Helpers.try_satisfy_any (T.unquote #(list (ty -> bool)) value) (T.unquote #ty ctr)) constructors in
+                        let filtered_constructor_qn = T.map (fun t -> Enum.unpack_enum_constructor (quote t)) filtered_constructor_term in
+                        T.map (fun n -> L.last n) filtered_constructor_qn
+                    in
+
+                    if op `Helpers.termeq` (`JsonStar.Schema.Dsl.allow) then Allow selected_constructors
+                    else if op `Helpers.termeq` (`JsonStar.Schema.Dsl.disallow) then Disallow selected_constructors
+                    else Helpers.tfail ("Unrecognized enum operator: " ^ (T.term_to_string op_with_arg))
+                    end
+                | _ -> Helpers.tfail ("Expected Tv_App. Got: " ^ (T.term_to_ast_string op_dsl))
+                end
+            end
+        | _ -> Helpers.tfail ((T.term_to_string t) ^ " expected to be of form Tv_App op value where op describes refinement and value is the value that should be used.")
+        end
     
